feat: add STLCProp.lean

Plfl/STLC.lean
@@ -1,21 +1,25 @@
+/-
+  Types and terms of the simply typed lambda calculus
+-/
 inductive Ty : Type
   | bool : Ty
   | arr : Ty → Ty → Ty
 
+notation "bool" => Ty.bool
+notation:70 τ₁ "⇒" τ₂ => Ty.arr τ₁ τ₂
+
+-- Decidable equality of types
 instance Ty.decEq : DecidableEq Ty
-  | Ty.bool , Ty.bool => isTrue rfl
-  | Ty.bool , Ty.arr _ _ => isFalse Ty.noConfusion
-  | Ty.arr _ _ , Ty.bool => isFalse Ty.noConfusion
-  | Ty.arr a₁ a₂ , Ty.arr b₁ b₂ =>
+  | bool , bool => isTrue rfl
+  | bool , _ ⇒ _ => isFalse Ty.noConfusion
+  | _ ⇒ _ , Ty.bool => isFalse Ty.noConfusion
+  | a₁ ⇒ a₂ , b₁ ⇒ b₂ =>
       match decEq a₁ b₁ with
       | isTrue h₁ =>
           match decEq a₂ b₂ with
           | isTrue h₂ => by rw [h₁, h₂]; apply isTrue; rfl
           | isFalse h₂ => by rw [h₁]; apply isFalse; intro h; cases h; apply h₂; rfl
       | isFalse h₁ => by apply isFalse; intro h; cases h; apply h₁; rfl
-
-notation "bool" => Ty.bool
-notation:7 τ₁ "⇒" τ₂ => Ty.arr τ₁ τ₂
 
 inductive Tm : Type
   | var : String → Tm
@@ -27,17 +31,19 @@ inductive Tm : Type
 
 notation "true" => Tm.tru
 notation "false" => Tm.fls
-notation:5 "λ" x ":" τ:8 "⇒" t:5 => Tm.lam x τ t
-notation:7 t₁:7 "⬝" t₂:8 => Tm.app t₁ t₂
+notation:50 "λ" x ":" τ:80 "⇒" t:50 => Tm.lam x τ t
+notation:70 t₁:70 "⬝" t₂:80 => Tm.app t₁ t₂
 notation "if" t₁ "then" t₂ "else" t₃ => Tm.ite t₁ t₂ t₃
 
 def notB : Tm := if true then false else true
 
+-- Values
 inductive Val : Tm → Prop
   | lam {x τ t} : Val (λ x : τ ⇒ t)
   | tru : Val Tm.tru
   | fls : Val Tm.fls
 
+-- Substitution
 def subst (x : String) (s : Tm) : Tm → Tm
   | Tm.var y => if x = y then s else Tm.var y
   | Tm.app t₁ t₂ => subst x s t₁ ⬝ subst x s t₂
@@ -46,23 +52,41 @@ def subst (x : String) (s : Tm) : Tm → Tm
   | Tm.fls => false
   | Tm.ite t₁ t₂ t₃ => if subst x s t₁ then subst x s t₂ else subst x s t₃
 
+notation:90 t "[" x "↦" s "]" => subst x s t
 
-notation:9 t "[" x "↦" s "]" => subst x s t
+/-
+  Reduction
+-/
+inductive Reduction : Tm → Tm → Prop
+  | app_abs {x τ t v} : Val v → Reduction ((λ x : τ ⇒ t) ⬝ v) (t [x ↦ v])
+  | app₁ {t₁ t₁' t₂} : Reduction t₁ t₁' → Reduction (t₁ ⬝ t₂) (t₁' ⬝ t₂)
+  | app₂ {v₁ t₂ t₂'} : Val v₁ → Reduction t₂ t₂' → Reduction (v₁ ⬝ t₂) (v₁ ⬝ t₂')
+  | tru {t₁ t₂} : Reduction (if true then t₁ else t₂) t₁
+  | fls {t₁ t₂} : Reduction (if false then t₁ else t₂) t₂
+  | ite {t₁ t₁' t₂ t₃} : Reduction t₁ t₁' → Reduction (if t₁ then t₂ else t₃) (if t₁' then t₂ else t₃)
 
+notation:40 t "—⟶" t' => Reduction t t'
+
+/-
+  Context management
+-/
 inductive Context : Type
   | empty : Context
   | cons : Context → String → Ty → Context
 
 notation "∅" => Context.empty
-notation:5 Γ ";" x ":" τ => Context.cons Γ x τ
+notation:50 Γ ";" x ":" τ => Context.cons Γ x τ
 
 inductive Lookup : Context → String → Ty → Prop
   | here {Γ x τ} : Lookup (Γ ; x : τ) x τ
   | there {Γ x y τ τ'} : x ≠ y → Lookup Γ x τ → Lookup (Γ ; y : τ') x τ
 
-notation:4 Γ "∋" x ":" τ => Lookup Γ x τ
+notation:40 Γ "∋" x ":" τ => Lookup Γ x τ
 
-inductive Judgement : Context → Tm → Ty → Type
+/-
+  Typing judgements
+-/
+inductive Judgement : Context → Tm → Ty → Prop
   | var {Γ x τ} : (Γ ∋ x : τ) → Judgement Γ (Tm.var x) τ
   | app {Γ t₁ t₂ τ τ'} : Judgement Γ t₁ (τ ⇒ τ') → Judgement Γ t₂ τ → Judgement Γ (t₁ ⬝ t₂) τ'
   | lam {Γ x τ t τ'} : Judgement (Γ ; x : τ) t τ' → Judgement Γ (λ x : τ ⇒ t) (τ ⇒ τ')
@@ -70,7 +94,7 @@ inductive Judgement : Context → Tm → Ty → Type
   | fls {Γ} : Judgement Γ Tm.fls bool
   | ite {Γ t₁ t₂ t₃ τ} : Judgement Γ t₁ bool → Judgement Γ t₂ τ → Judgement Γ t₃ τ → Judgement Γ (if t₁ then t₂ else t₃) τ
 
-notation:4 Γ "⊢" t ":" τ => Judgement Γ t τ
+notation:40 Γ "⊢" t ":" τ => Judgement Γ t τ
 
 theorem lookup_is_functional {Γ x τ τ'} : (Γ ∋ x : τ) → (Γ ∋ x : τ') → τ = τ'
   | Lookup.here , Lookup.here => rfl
