Plfl/STLCProp.lean
@@ -1,0 +1,132 @@
+import Plfl.STLC
+
+/-
+  Theorem: Canonical Forms
+
+  If Γ ⊢ t : τ and t is a value, then one of the following holds:
+
+  1. t = true
+  2. t = false
+  3. t = λx:τ'.t'
+-/
+theorem canonical_forms_bool
+  : ∀ t, (∅ ⊢ t : bool) → Val t → t = true ∨ t = false
+  := by
+    intros t ht hv
+    cases hv with
+    | tru => simp
+    | fls => simp
+    | lam => cases ht
+
+theorem canonical_forms_lam
+  : ∀ t τ₁ τ₂, (∅ ⊢ t : τ₁ ⇒ τ₂) → Val t → ∃ x t', t = (λ x : τ₁ ⇒ t')
+  := by
+    intros t τ₁ τ₂ ht hv
+    cases hv with
+    | tru => cases ht
+    | fls => cases ht
+    | @lam x _ t =>
+        simp
+        cases ht
+        apply (Exists.intro x ∘ Exists.intro t)
+        simp
+
+/- Theorem progress : ∀ t T,
+  empty |-- t \in T →
+  value t ∨ ∃ t', t --> t'. -/
+
+theorem progress : ∀ t τ, (∅ ⊢ t : τ) → Val t ∨ (∃ t', t —⟶ t') := by
+  intro t τ ht
+  cases ht with
+  | var x =>
+      apply Or.inl
+      contradiction
+  | @app _ t₁ t₂ τ₁ _ ht₁ ht₂ =>
+      have ht₁' := progress t₁ (τ₁⇒τ) ht₁
+      cases ht₁' with
+      | inl hv₁ =>
+          have ht₂' := progress t₂ τ₁ ht₂
+          cases ht₂' with
+          | inl hv₂ =>
+              apply Or.inr
+              cases hv₁ with
+              | @lam x _ t =>
+                  exists (t [x ↦ t₂])
+                  apply (Reduction.app_abs hv₂)
+              | tru => cases ht₁
+              | fls => cases ht₁
+          | inr hstep₂ =>
+              apply Or.inr
+              have ⟨t₂', hstep₂'⟩ := hstep₂
+              exists (t₁ ⬝ t₂')
+              apply (Reduction.app₂ hv₁ hstep₂')
+      | inr hstep₁ =>
+          apply Or.inr
+          have ⟨t₁', hstep₁'⟩ := hstep₁
+          exists (t₁' ⬝ t₂)
+          apply (Reduction.app₁ hstep₁')
+  | lam ht => apply Or.inl Val.lam
+  | tru => apply Or.inl Val.tru
+  | fls => apply Or.inl Val.fls
+  | @ite _ t₁ t₂ t₃ _ ht₁ ht₂ ht₃ =>
+      have ht₁' := progress t₁ bool ht₁
+      cases ht₁' with
+      | inl hv₁ =>
+          cases hv₁ with
+          | tru => apply Or.inr (Exists.intro t₂ Reduction.tru)
+          | fls => apply Or.inr (Exists.intro t₃ Reduction.fls)
+          | lam => cases ht₁
+      | inr hstep₁ =>
+          apply Or.inr
+          have ⟨t₁', hstep₁'⟩ := hstep₁
+          apply (Exists.intro (if t₁' then t₂ else t₃) (Reduction.ite hstep₁'))
+termination_by progress t _ _  => t
+
+-- Lemma: Weekening
+theorem weakening : ∀ Γ Γ' t τ, (Γ ⊂ Γ') → (Γ ⊢ t : τ) → Γ' ⊢ t : τ := by
+  intro Γ Γ' t τ hsub ht
+  induction ht with
+  | var x =>
+      cases hsub
+      apply Ty.var
+      assumption
+  | app ht₁ ht₂ =>
+      cases hsub
+      apply Ty.app
+      apply ht₁
+      apply ht₂
+  | lam ht =>
+      cases hsub
+      apply Ty.lam
+      apply ht
+  | tru =>
+      cases hsub
+      apply Ty.tru
+  | fls =>
+      cases hsub
+      apply Ty.fls
+  | ite ht₁ ht₂ ht₃ =>
+      cases hsub
+      apply Ty.ite
+      apply ht₁
+      apply ht₂
+      apply ht₃
+
+/-
+  Theorem: Preservation
+
+  If Γ ⊢ t : τ and t —⟶ t', then Γ ⊢ t' : τ.
+-/
+theorem preservation : ∀ t t' τ, (∅ ⊢ t : τ) → (t —⟶ t') → ∅ ⊢ t' : τ := by
+  intro t t' τ ht hstep
+  cases ht with
+  | var x => cases hstep
+  | app ht₁ ht₂ =>
+      cases hstep with
+      | app_abs hv => sorry
+      | app₁ ht₁' => sorry
+      | app₂ hv₁ ht₂' => sorry
+  | lam ht => cases hstep
+  | tru => cases hstep
+  | fls => cases hstep
+  | ite t₁ t₂ t₃ => sorry
